update instantiation proofs

dsn/Lang/Typing/Basic.lean
@@ -41,72 +41,72 @@ theorem Stable.subject_expansion :
 
 
 mutual
-  def Subtyping (am : List (String × (Expr → Prop))) (left : Typ) (right : Typ) : Prop :=
-    ∀ e, Typing am e left → Typing am e right
+  def Subtyping (tmp : String) (am : List (String × (Expr → Prop))) (left : Typ) (right : Typ) : Prop :=
+    ∀ e, Typing tmp am e left → Typing tmp am e right
   termination_by (Typ.size left + Typ.size right, 0)
   decreasing_by
     all_goals (apply Prod.Lex.left ; simp [Typ.zero_lt_size])
 
 
-  def MultiSubtyping (am : List (String × (Expr → Prop))) : List (Typ × Typ) → Prop
+  def MultiSubtyping (tmp : String) (am : List (String × (Expr → Prop))) : List (Typ × Typ) → Prop
   | .nil => True
   | .cons (left, right) remainder =>
-    Subtyping am left right ∧ MultiSubtyping am remainder
+    Subtyping tmp am left right ∧ MultiSubtyping tmp am remainder
   termination_by sts => (List.pair_typ_size sts, 0)
   decreasing_by
     all_goals (apply Prod.Lex.left ; simp [List.pair_typ_size, List.pair_typ_zero_lt_size, Typ.zero_lt_size])
 
-  def PosMonotonic (name : String) (am : List (String × (Expr → Prop))) (t : Typ) : Prop :=
+  def PosMonotonic (name : String) (tmp : String) (am : List (String × (Expr → Prop))) (t : Typ) : Prop :=
     (∀ P0 P1 : Expr → Prop,
       Stable P0 → Stable P1 →
       (∀ e, P0 e → P1 e) →
-      (∀ e , Typing ((name,P0)::am) e t → Typing ((name,P1)::am) e t)
+      (∀ e , Typing tmp ((name,P0)::am) e t → Typing tmp ((name,P1)::am) e t)
     )
   termination_by (Typ.size t, 1)
 
 
   -- TODO: need to add a tvars field for named instantiation
-  def Typing (am : List (String × (Expr → Prop))) (e : Expr) : Typ → Prop
+  def Typing (tmp : String) (am : List (String × (Expr → Prop))) (e : Expr) : Typ → Prop
   | .var id => Safe e ∧ ∃ P, Stable P ∧ Prod.find id am = some P ∧ P e
   | .bvar _ => False
   | .bot => False
   | .top => Safe e
-  | .iso l t => Safe e ∧ Typing am (.extract e l) t
-  | .entry l t => Safe e ∧ Typing am (.project e l) t
+  | .iso l t => Safe e ∧ Typing tmp am (.extract e l) t
+  | .entry l t => Safe e ∧ Typing tmp am (.project e l) t
   | .path left right =>
     Safe e ∧
-    ∀ arg , Typing am arg left → Typing am (.app e arg) right
-  | .unio left right => Typing am e left ∨ Typing am e right
-  | .inter left right => Typing am e left ∧ Typing am e right
-  | .diff left right => Typing am e left ∧ ¬ (Typing am e right)
+    ∀ arg , Typing tmp am arg left → Typing tmp am (.app e arg) right
+  | .unio left right => Typing tmp am e left ∨ Typing tmp am e right
+  | .inter left right => Typing tmp am e left ∧ Typing tmp am e right
+  | .diff left right => Typing tmp am e left ∧ ¬ (Typing tmp am e right)
 
   | .exi bs cs body =>
     (∀ a ∈ bs , a = "") ∧
     ∀ names,
     List.length names = List.length bs →
-    List.Disjoint names (Typ.list_prod_free_vars cs ++ Typ.free_vars body) →
+    List.Disjoint names (tmp :: Typ.list_prod_free_vars cs ++ Typ.free_vars body) →
       ∃ am' , Prod.dom am' = names ∧
-      (MultiSubtyping (am' ++ am) (Typ.constraints_instantiate 0 (List.map Typ.var names) cs)) ∧
-      (Typing (am' ++ am) e (Typ.instantiate 0 (List.map Typ.var names) body))
+      (MultiSubtyping tmp (am' ++ am) (Typ.constraints_instantiate 0 (List.map Typ.var names) cs)) ∧
+      (Typing tmp (am' ++ am) e (Typ.instantiate 0 (List.map Typ.var names) body))
 
   | .all bs cs body =>
     Safe e ∧
     (∀ a ∈ bs , a = "") ∧
     ∃ names,
     List.length names = List.length bs ∧
-    List.Disjoint names (Typ.list_prod_free_vars cs ++ Typ.free_vars body) ∧
+    List.Disjoint names (tmp :: Typ.list_prod_free_vars cs ++ Typ.free_vars body) ∧
     ∀ am' , Prod.dom am' = names →
-    (MultiSubtyping (am' ++ am) (Typ.constraints_instantiate 0 (List.map Typ.var names) cs)) →
-      (Typing (am' ++ am) e (Typ.instantiate 0 (List.map Typ.var names) body))
+    (MultiSubtyping tmp (am' ++ am) (Typ.constraints_instantiate 0 (List.map Typ.var names) cs)) →
+      (Typing tmp (am' ++ am) e (Typ.instantiate 0 (List.map Typ.var names) body))
   | .lfp a body =>
     Safe e ∧
     a = "" ∧
-    ∀ name , name ∉ (Typ.free_vars body) →
-      PosMonotonic name am (Typ.instantiate 0 [.var name] body) ∧
+    ∀ name , name ∉ (tmp :: Typ.free_vars body) →
+      PosMonotonic name tmp am (Typ.instantiate 0 [.var name] body) ∧
       /- infimum of -/
       (∀ P, Stable P →
         /- pre-fixed point -/
-        (∀ e', Typing ((name,P) :: am) e' (Typ.instantiate 0 [.var name] body) → P e') →
+        (∀ e', Typing tmp ((name,P) :: am) e' (Typ.instantiate 0 [.var name] body) → P e') →
         P e
       )
   termination_by t => (Typ.size t, 0)
@@ -122,31 +122,31 @@ mutual
 end
 
 
-def NegMonotonic (name : String) (am : List (String × (Expr → Prop))) (t : Typ) : Prop :=
+def NegMonotonic (name : String) (tmp : String) (am : List (String × (Expr → Prop))) (t : Typ) : Prop :=
   (∀ P0 P1 : Expr → Prop,
     Stable P0 → Stable P1 →
     (∀ e, P0 e → P1 e) →
-    (∀ e , Typing ((name,P1)::am) e t → Typing ((name,P0)::am) e t)
+    (∀ e , Typing tmp ((name,P1)::am) e t → Typing tmp ((name,P0)::am) e t)
   )
 
-def Monotonic (polarity : Bool) (name : String) (am : List (String × (Expr → Prop))) (t : Typ) : Prop :=
-  (polarity = true ∧ PosMonotonic name am t) ∨
-  (polarity = false ∧ NegMonotonic name am t)
+def Monotonic (polarity : Bool) (name : String) (tmp : String) (am : List (String × (Expr → Prop))) (t : Typ) : Prop :=
+  (polarity = true ∧ PosMonotonic name tmp am t) ∨
+  (polarity = false ∧ NegMonotonic name tmp am t)
 
-def MultiMonotonic (polarity : Bool) (name : String) (am : List (String × (Expr → Prop))) (cs : List (Typ × Typ)) : Prop :=
-  ∀ lower upper, (lower,upper) ∈ cs → Monotonic (not polarity) name am lower ∧ Monotonic polarity name am upper
+def MultiMonotonic (polarity : Bool) (name : String) (tmp : String) (am : List (String × (Expr → Prop))) (cs : List (Typ × Typ)) : Prop :=
+  ∀ lower upper, (lower,upper) ∈ cs → Monotonic (not polarity) name tmp am lower ∧ Monotonic polarity name tmp am upper
 
-def EitherMultiMonotonic (name : String) (am : List (String × (Expr → Prop))) (cs : List (Typ × Typ)) : Prop :=
-  MultiMonotonic .true name am cs ∨ MultiMonotonic .false name am cs
+def EitherMultiMonotonic (name : String) (tmp : String) (am : List (String × (Expr → Prop))) (cs : List (Typ × Typ)) : Prop :=
+  MultiMonotonic .true name tmp am cs ∨ MultiMonotonic .false name tmp am cs
 
 
 def MultiTyping
-  (tam : List (String × (Expr → Prop))) (eam : List (String × Expr)) (context : List (String × Typ)) : Prop
-:= ∀ {x t}, Prod.find x context = .some t → ∃ e, (Prod.find x eam) = .some e ∧ Typing tam e t
+  (tmp : String) (tam : List (String × (Expr → Prop))) (eam : List (String × Expr)) (context : List (String × Typ)) : Prop
+:= ∀ {x t}, Prod.find x context = .some t → ∃ e, (Prod.find x eam) = .some e ∧ Typing tmp tam e t
 
 
 theorem Typing.safety :
-  Typing am e t → Safe e
+  Typing tmp am e t → Safe e
 := by cases t with
 | bvar i =>
   simp [Typing]
@@ -188,17 +188,17 @@ theorem Typing.safety :
   apply Typing.safety h0
 | all bs cs body =>
   simp [Typing]
-  intro h0 h1 names h2 h3 h4 h5
+  intro h0 h1 names h2 h3 h4 h5 h6
   exact h0
 | exi bs cs body =>
   simp [Typing]
   intro h0 h1 e' h2
-  have ⟨names,h3,h4⟩ := String.fresh_names (List.length bs) (Typ.list_prod_free_vars cs ++ Typ.free_vars body)
+  have ⟨names,h3,h4⟩ := String.fresh_names (List.length bs) (tmp :: Typ.list_prod_free_vars cs ++ Typ.free_vars body)
   simp at h4
-  have ⟨h4A,h4B⟩ := h4
+  have ⟨h4A,h4B,h4C⟩ := h4
 
 
-  have ⟨am',h5,h6,h7⟩ := h1 names h3 h4A h4B
+  have ⟨am',h5,h6,h7⟩ := h1 names h3 h4A h4B h4C
   apply Typing.safety h7 _ h2
 | lfp x body =>
   simp [Typing]
@@ -219,7 +219,7 @@ decreasing_by
 
 
 theorem Typing.progress :
-  Typing am e t → Expr.valued e ∨ ∃ e', NStep e e'
+  Typing tmp am e t → Expr.valued e ∨ ∃ e', NStep e e'
 := by
   intro h0
   apply Safe.progress
@@ -229,7 +229,7 @@ theorem Typing.progress :
 mutual
   theorem Typing.subject_reduction
     (transition : NStep e e')
-  : Typing am e t → Typing am e' t
+  : Typing tmp am e t → Typing tmp am e' t
   := by cases t with
   | bvar i =>
     simp [Typing]
@@ -304,15 +304,15 @@ mutual
     simp [Typing]
     intro h0 h1
     apply And.intro h0
-    intro names h3 h4A h4B
-    have ⟨am',h5,h6,h7⟩ := h1 names h3 h4A h4B
+    intro names h3 h4A h4B h4C
+    have ⟨am',h5,h6,h7⟩ := h1 names h3 h4A h4B h4C
     exists am'
     simp [*]
     apply Typing.subject_reduction transition h7
 
   | all bs quals body =>
     simp [Typing]
-    intro h0 h1 names h2 h3A h3B h4
+    intro h0 h1 names h2 h3A h3B h3C h4
     apply And.intro
     { apply Safe.subject_reduction transition h0 }
     { apply And.intro h1
@@ -329,8 +329,8 @@ mutual
     apply And.intro
     { exact Safe.subject_reduction transition safe }
     { apply And.intro nameless
-      intro name h1
-      have ⟨h2,h3⟩ := h0 name h1
+      intro name h1A h1B
+      have ⟨h2,h3⟩ := h0 name h1A h1B
       apply And.intro h2
       intro P h4 h5
       apply Stable.subject_reduction h4 transition
@@ -360,7 +360,7 @@ mutual
 
   theorem Typing.subject_expansion
     (transition : NStep e e')
-  : Typing am e' t → Typing am e t
+  : Typing tmp am e' t → Typing tmp am e t
   := by cases t with
   | bvar i =>
     simp [Typing]
@@ -435,15 +435,15 @@ mutual
     simp [Typing]
     intro h0 h1
     apply And.intro h0
-    intro names h3 h4A h4B
-    have ⟨am',h5,h6,h7⟩ := h1 names h3 h4A h4B
+    intro names h3 h4A h4B h4C
+    have ⟨am',h5,h6,h7⟩ := h1 names h3 h4A h4B h4C
     exists am'
     simp [*]
     apply Typing.subject_expansion transition h7
 
   | all bs cs body =>
     simp [Typing]
-    intro h0 h1 names h2 h3A h3B h4
+    intro h0 h1 names h2 h3A h3B h3C h4
     apply And.intro
     { apply Safe.subject_expansion transition h0 }
     { apply And.intro h1
@@ -460,8 +460,8 @@ mutual
     apply And.intro
     { exact Safe.subject_expansion transition safe }
     { apply And.intro nameless
-      intro name h1
-      have ⟨h2,h3⟩ := h0 name h1
+      intro name h1A h1B
+      have ⟨h2,h3⟩ := h0 name h1A h1B
       apply And.intro h2
       intro P h4 h5
       apply Stable.subject_expansion h4 transition
@@ -504,7 +504,7 @@ end
 
 theorem Typing.refl_trans_left_subject_expansion
   (transition : ReflTransLeft NStep e e')
-: Typing am e' t → Typing am e t
+: Typing tmp am e' t → Typing tmp am e t
 := by induction transition with
 | refl =>
   intro h0 ; exact h0
@@ -515,14 +515,14 @@ theorem Typing.refl_trans_left_subject_expansion
 
 theorem Typing.refl_trans_subject_expansion
   (transition : ReflTrans NStep e e')
-: Typing am e' t → Typing am e t
+: Typing tmp am e' t → Typing tmp am e t
 := by
   apply Typing.refl_trans_left_subject_expansion
   exact ReflTrans.reverse transition
 
 theorem Typing.refl_trans_subject_reduction
   (transition : ReflTrans NStep e e')
-: Typing am e t → Typing am e' t
+: Typing tmp am e t → Typing tmp am e' t
 := by induction transition with
 | refl =>
   intro h0 ; exact h0
@@ -537,8 +537,8 @@ mutual
 
   theorem Subtyping.env_insert_reflection :
     (name ∉ Typ.free_vars lower ∧ name ∉ Typ.free_vars upper ∨ name ∈ Prod.dom m0) →
-    Subtyping (m0 ++ (name,P) :: m1) lower upper →
-    Subtyping (m0 ++ m1) lower upper
+    Subtyping tmp (m0 ++ (name,P) :: m1) lower upper →
+    Subtyping tmp (m0 ++ m1) lower upper
   := by
     simp [Subtyping]
     intro h0 h1 e h2
@@ -552,8 +552,8 @@ mutual
 
   theorem Subtyping.env_insert_preservation :
     (name ∉ Typ.free_vars lower ∧ name ∉ Typ.free_vars upper ∨ name ∈ Prod.dom m0) →
-    Subtyping (m0 ++ m1) lower upper →
-    ∀ P, Subtyping (m0 ++ (name,P) :: m1) lower upper
+    Subtyping tmp (m0 ++ m1) lower upper →
+    ∀ P, Subtyping tmp (m0 ++ (name,P) :: m1) lower upper
   := by
     simp [Subtyping]
     intro h0 h1 P e h2
@@ -568,8 +568,8 @@ mutual
 
   theorem MultiSubtyping.env_insert_reflection :
     (name ∉ Typ.list_prod_free_vars cs ∨ name ∈ Prod.dom m0) →
-    MultiSubtyping (m0 ++ (name,P) :: m1) cs →
-    MultiSubtyping (m0 ++ m1) cs
+    MultiSubtyping tmp (m0 ++ (name,P) :: m1) cs →
+    MultiSubtyping tmp (m0 ++ m1) cs
   := by cases cs with
   | nil =>
     simp [MultiSubtyping]
@@ -587,8 +587,8 @@ mutual
 
   theorem MultiSubtyping.env_insert_preservation :
     (name ∉ Typ.list_prod_free_vars cs ∨ name ∈ Prod.dom m0) →
-    MultiSubtyping (m0 ++ m1) cs →
-    ∀ P, MultiSubtyping (m0 ++ (name,P) :: m1) cs
+    MultiSubtyping tmp (m0 ++ m1) cs →
+    ∀ P, MultiSubtyping tmp (m0 ++ (name,P) :: m1) cs
   := by cases cs with
   | nil =>
     simp [MultiSubtyping]
@@ -607,8 +607,8 @@ mutual
 
   theorem PosMonotonic.env_insert_reflection :
     (name ∉ Typ.free_vars t ∨ name = point ∨ name ∈ Prod.dom m0)  →
-    PosMonotonic point (m0 ++ (name,P) :: m1) t →
-    PosMonotonic point (m0 ++ m1) t
+    PosMonotonic point tmp (m0 ++ (name,P) :: m1) t →
+    PosMonotonic point tmp (m0 ++ m1) t
   := by
     simp [PosMonotonic]
     intro h0 h1 P0 P1 stable0 stable1 h3 e h5
@@ -633,8 +633,8 @@ mutual
 
   theorem PosMonotonic.env_insert_preservation :
     (name ∉ Typ.free_vars t ∨ name = point ∨ name ∈ Prod.dom m0)  →
-    PosMonotonic point (m0 ++ m1) t →
-    ∀ P, PosMonotonic point (m0 ++ (name,P) :: m1) t
+    PosMonotonic point tmp (m0 ++ m1) t →
+    ∀ P, PosMonotonic point tmp (m0 ++ (name,P) :: m1) t
   := by
     simp [PosMonotonic]
     intro h0 h1 P0 P1 P stable0 stable1 h3 e h5
@@ -661,8 +661,8 @@ mutual
 
   theorem Typing.env_insert_reflection :
     (name ∉ Typ.free_vars t ∨ name ∈ Prod.dom m0) →
-    Typing (m0 ++ (name,P) :: m1) e t →
-    Typing (m0 ++ m1) e t
+    Typing tmp (m0 ++ (name,P) :: m1) e t →
+    Typing tmp (m0 ++ m1) e t
   := by cases t with
   | bvar i =>
     simp [Typing]
@@ -747,7 +747,7 @@ mutual
 
   | all bs cs body =>
     simp [Typing, Typ.free_vars]
-    intro h0 h1 h2 names h3 h4A h4B h5
+    intro h0 h1 h2 names h3 h4A h4B h4C h5
     simp [*]
     apply And.intro h2
     exists names
@@ -824,9 +824,9 @@ mutual
     simp [Typing, Typ.free_vars]
     intro h0 h1 h2
     apply And.intro h1
-    intro names h5 h6A h6B
+    intro names h5 h6A h6B h6C
 
-    have ⟨m,h9,h10,h11⟩ := h2 names h5 h6A h6B
+    have ⟨m,h9,h10,h11⟩ := h2 names h5 h6A h6B h6C
     exists m
     simp [*]
     have ⟨h12,h13⟩ := Iff.mp and_or_right h0
@@ -896,9 +896,9 @@ mutual
     simp [Typing, Typ.free_vars]
     intro h0 h1 h2 h3
     simp [*]
-    intro name' h4
+    intro name' h4A h4B
 
-    have ⟨h6,h7⟩ := h3 name' h4
+    have ⟨h6,h7⟩ := h3 name' h4A h4B
 
     apply And.intro
     { apply @PosMonotonic.env_insert_reflection _ name
@@ -950,8 +950,8 @@ mutual
 
   theorem Typing.env_insert_preservation :
     (name ∉ Typ.free_vars t ∨ name ∈ Prod.dom m0) →
-    Typing (m0 ++ m1) e t →
-    ∀ P, Typing (m0 ++ (name,P) :: m1) e t
+    Typing tmp (m0 ++ m1) e t →
+    ∀ P, Typing tmp (m0 ++ (name,P) :: m1) e t
   := by cases t with
   | bvar i =>
     simp [Typing]
@@ -1034,7 +1034,7 @@ mutual
 
   | all bs cs body =>
     simp [Typing, Typ.free_vars]
-    intro h0 h1 h2 names h3 h4A h4B h5 P
+    intro h0 h1 h2 names h3 h4A h4B h4C h5 P
     simp [*]
     apply And.intro h2
     exists names
@@ -1111,9 +1111,9 @@ mutual
     simp [Typing, Typ.free_vars]
     intro h0 h1 h2 P
     apply And.intro h1
-    intro names h5 h6A h6B
+    intro names h5 h6A h6B h6C
 
-    have ⟨m,h9,h10,h11⟩ := h2 names h5 h6A h6B
+    have ⟨m,h9,h10,h11⟩ := h2 names h5 h6A h6B h6C
     exists m
     simp [*]
     have ⟨h12,h13⟩ := Iff.mp and_or_right h0
@@ -1183,9 +1183,9 @@ mutual
     simp [Typing, Typ.free_vars]
     intro h0 h1 h2 h3 P
     simp [*]
-    intro name' h4
+    intro name' h4A h4B
 
-    have ⟨h6,h7⟩ := h3 name' h4
+    have ⟨h6,h7⟩ := h3 name' h4A h4B
 
     apply And.intro
     { apply @PosMonotonic.env_insert_preservation _ name
@@ -1238,8 +1238,8 @@ end
 
 theorem Typing.env_cons_suffix_preservation :
   name ∉ Typ.free_vars t →
-  Typing m e t →
-  ∀ P, Typing ((name,P) :: m) e t
+  Typing tmp m e t →
+  ∀ P, Typing tmp ((name,P) :: m) e t
 := by
   intro h0 h1 P
   have h2 : (name,P) :: m = [] ++ (name,P) :: m  := by rfl
@@ -1250,8 +1250,8 @@ theorem Typing.env_cons_suffix_preservation :
 
 theorem Typing.env_cons_suffix_reflection :
   name ∉ Typ.free_vars t →
-  Typing ((name,P) :: m) e t →
-  Typing m e t
+  Typing tmp ((name,P) :: m) e t →
+  Typing tmp m e t
 := by
   intro h0 h1
   have h2 : m = [] ++ m  := by rfl
@@ -1262,8 +1262,8 @@ theorem Typing.env_cons_suffix_reflection :
 
 theorem Typing.env_append_suffix_preservation :
   List.Disjoint (Prod.dom m0) (Typ.free_vars t) →
-  Typing m1 e t →
-  Typing (m0 ++ m1) e t
+  Typing tmp m1 e t →
+  Typing tmp (m0 ++ m1) e t
 := by induction m0 with
 | nil =>
   simp [List.Disjoint]
@@ -1278,8 +1278,8 @@ theorem Typing.env_append_suffix_preservation :
 
 theorem Typing.env_append_suffix_reflection :
   List.Disjoint (Prod.dom m0) (Typ.free_vars t) →
-  Typing (m0 ++ m1) e t →
-  Typing m1 e t
+  Typing tmp (m0 ++ m1) e t →
+  Typing tmp m1 e t
 := by induction m0 with
 | nil =>
   simp [List.Disjoint]
@@ -1295,8 +1295,8 @@ theorem Typing.env_append_suffix_reflection :
 
 theorem Typing.env_preservation :
   Typ.free_vars t = [] →
-  Typing [] e t →
-  Typing m e t
+  Typing tmp [] e t →
+  Typing tmp m e t
 := by
   intro h0 h1
   have h2 : m = m ++ [] := by exact Eq.symm (List.append_nil m)
@@ -1307,8 +1307,8 @@ theorem Typing.env_preservation :
 
 theorem Typing.env_reflection :
   Typ.free_vars t = [] →
-  Typing m e t →
-  Typing [] e t
+  Typing tmp m e t →
+  Typing tmp [] e t
 := by
   intro h0 h1
   have h2 : m = m ++ [] := by exact Eq.symm (List.append_nil m)
