dsn/Lang/Typing/Instantiation.lean
@@ -21,59 +21,33 @@ mutual
 
 
   theorem Subtyping.generalized_nameless_instantiation :
-    Typ.free_vars t ⊆ Prod.dom am →
-    List.Disjoint (Prod.dom am') (Prod.dom am) →
     name ∉ Prod.dom am' →
-    name ∉ Prod.dom am →
+    Typ.free_vars t = [] →
     Typ.wellformed t →
-    Subtyping (am' ++ (name,fun e => Typing am e t) :: am) (Typ.instantiate depth [.var name] lower) (Typ.instantiate depth [.var name] upper) →
-    Subtyping (am' ++ (name,fun e => Typing am e t) :: am) (Typ.instantiate depth [t] lower) (Typ.instantiate depth [t] upper)
+    Subtyping name (am' ++ (name,fun e => Typing name [] e t) :: am) (Typ.instantiate depth [.var name] lower) (Typ.instantiate depth [.var name] upper) →
+    Subtyping name (am' ++ (name,fun e => Typing name [] e t) :: am) (Typ.instantiate depth [t] lower) (Typ.instantiate depth [t] upper)
   := by
-    simp [Subtyping, Prod.dom]
-    intro h2 h3 h4 h5 wf h6
-    { intro e h8
-      apply Typing.generalized_nameless_instantiation h2 h3
-      { simp [Prod.dom]; exact h4 }
-      { simp [Prod.dom]; exact h5 }
-      { exact wf }
-      {
-        apply h6
-        apply Typing.generalized_named_instantiation h2 h3
-        { simp [Prod.dom]; exact h4 }
-        { simp [Prod.dom]; exact h5 }
-        { exact wf }
-        { exact h8 }
-      }
-    }
+    simp [Subtyping]
+    intro h2 h3 h4 h5 e h6
+    apply Typing.generalized_nameless_instantiation h2 h3 h4
+    apply h5
+    apply Typing.generalized_named_instantiation h2 h3 h4 h6
   termination_by (Typ.size lower + Typ.size upper, 0)
   decreasing_by
     all_goals (apply Prod.Lex.left ; simp [Typ.zero_lt_size])
 
   theorem Subtyping.generalized_named_instantiation :
-    Typ.free_vars t ⊆ Prod.dom am →
-    List.Disjoint (Prod.dom am') (Prod.dom am) →
     name ∉ Prod.dom am' →
-    name ∉ Prod.dom am →
+    Typ.free_vars t = [] →
     Typ.wellformed t →
-    Subtyping (am' ++ (name,fun e => Typing am e t) :: am) (Typ.instantiate depth [t] lower) (Typ.instantiate depth [t] upper) →
-    Subtyping (am' ++ (name,fun e => Typing am e t) :: am) (Typ.instantiate depth [.var name] lower) (Typ.instantiate depth [.var name] upper)
+    Subtyping name (am' ++ (name,fun e => Typing name [] e t) :: am) (Typ.instantiate depth [t] lower) (Typ.instantiate depth [t] upper) →
+    Subtyping name (am' ++ (name,fun e => Typing name [] e t) :: am) (Typ.instantiate depth [.var name] lower) (Typ.instantiate depth [.var name] upper)
   := by
-    simp [Subtyping, Prod.dom]
-    intro h2 h3 h4 h5 wf h6
-    { intro e h8
-      apply Typing.generalized_named_instantiation h2 h3
-      { simp [Prod.dom]; exact h4 }
-      { simp [Prod.dom]; exact h5 }
-      { exact wf }
-      {
-        apply h6
-        apply Typing.generalized_nameless_instantiation h2 h3
-        { simp [Prod.dom]; exact h4 }
-        { simp [Prod.dom]; exact h5 }
-        { exact wf }
-        { exact h8 }
-      }
-    }
+    simp [Subtyping]
+    intro h2 h3 h4 h5 e h6
+    apply Typing.generalized_named_instantiation h2 h3 h4
+    apply h5
+    apply Typing.generalized_nameless_instantiation h2 h3 h4 h6
   termination_by (Typ.size lower + Typ.size upper, 0)
   decreasing_by
     all_goals (apply Prod.Lex.left ; simp [Typ.zero_lt_size])
@@ -82,423 +56,324 @@ mutual
 
 
   theorem PosMonotonic.generalized_nameless_instantiation :
-    Typ.free_vars t ⊆ Prod.dom am →
-    List.Disjoint (Prod.dom am') (Prod.dom am) →
     name ∉ Prod.dom am' →
-    name ∉ Prod.dom am →
+    Typ.free_vars t = [] →
     Typ.wellformed t →
-    point ∉ Prod.dom am' →
-    point ≠ name →
-    point ∉ Prod.dom am →
-    PosMonotonic point (am' ++ (name,fun e => Typing am e t) :: am) (Typ.instantiate depth [.var name] body) →
-    PosMonotonic point (am' ++ (name,fun e => Typing am e t) :: am) (Typ.instantiate depth [t] body)
+    name ≠ point →
+    PosMonotonic point name (am' ++ (name,fun e => Typing name [] e t) :: am) (Typ.instantiate depth [.var name] body) →
+    PosMonotonic point name (am' ++ (name,fun e => Typing name [] e t) :: am) (Typ.instantiate depth [t] body)
   := by
-    simp [PosMonotonic, Prod.dom]
-    intro h1 h2 h3 h4 wf _ h6 h7 h8 P0 P1 stable_P0 stable_P1 h9 e h10
-    -- h5 h6 h7
-    have h11 :
-      (point, P1) :: (am' ++ (name, fun e => Typing am e t) :: am) =
-      ((point, P1) :: am') ++ (name, fun e => Typing am e t) :: am
-    := by rfl
-
-    rw [h11]
-    apply Typing.generalized_nameless_instantiation h1
-    {
-      simp [List.Disjoint, Prod.dom]
-      apply And.intro h7
-      simp [List.Disjoint] at h2
-      exact h2
+    simp [PosMonotonic]
+    intro h1 h2 h3
+    intro h5
+    intro h7 P0 P1 stable_P0 stable_P1 h9 e h10
+    rw [←List.cons_append]
+    apply Typing.generalized_nameless_instantiation
+    { simp [Prod.dom] at h1
+      simp [Prod.dom,h1,h5]
     }
-    { simp [Prod.dom]
-      apply And.intro
-      { intro h12 ; exact h6 (Eq.symm h12) }
+    { exact h2 }
+    { exact h3 }
+    { simp
+      apply h7 _ _ stable_P0 stable_P1 h9
+      rw [←List.cons_append]
+      apply Typing.generalized_named_instantiation
+      { simp [Prod.dom] at h1
+        simp [Prod.dom,h1,h5]
+      }
+      { exact h2 }
       { exact h3 }
-    }
-    { simp [Prod.dom] ; exact h4 }
-    { exact wf }
-    {
-      simp
-      apply h8 _ _ stable_P0 stable_P1 h9
-
-      have h12 :
-        (point, P0) :: (am' ++ (name, fun e => Typing am e t) :: am) =
-        ((point, P0) :: am') ++ (name, fun e => Typing am e t) :: am
-      := by rfl
-
-      rw [h12]
-      apply Typing.generalized_named_instantiation h1
-      {
-        simp [List.Disjoint, Prod.dom]
-        apply And.intro h7
-        simp [List.Disjoint] at h2
-        exact h2
-      }
-      { simp [Prod.dom]
-        apply And.intro
-        { intro h12 ; exact h6 (Eq.symm h12) }
-        { exact h3 }
-      }
-      { simp [Prod.dom] ; exact h4 }
-      { exact wf }
       { exact h10 }
     }
   termination_by (Typ.size body, 1)
 
   theorem PosMonotonic.generalized_named_instantiation :
-    Typ.free_vars t ⊆ Prod.dom am →
-    List.Disjoint (Prod.dom am') (Prod.dom am) →
     name ∉ Prod.dom am' →
-    name ∉ Prod.dom am →
+    Typ.free_vars t = [] →
     Typ.wellformed t →
-    point ∉ Prod.dom am' →
-    point ≠ name →
-    point ∉ Prod.dom am →
-    PosMonotonic point (am' ++ (name,fun e => Typing am e t) :: am) (Typ.instantiate depth [t] body) →
-    PosMonotonic point (am' ++ (name,fun e => Typing am e t) :: am) (Typ.instantiate depth [.var name] body)
+    name ≠  point →
+    PosMonotonic point name (am' ++ (name,fun e => Typing name [] e t) :: am) (Typ.instantiate depth [t] body) →
+    PosMonotonic point name (am' ++ (name,fun e => Typing name [] e t) :: am) (Typ.instantiate depth [.var name] body)
   := by
-    simp [PosMonotonic, Prod.dom]
-    intro h1 h2 h3 h4 wf h5 h6 h7 h8 P0 P1 stable_P0 stable_P1 h9 e h10
+    simp [PosMonotonic]
+    intro h1 h2 h3
+    intro h5
+    intro h7 P0 P1 stable_P0 stable_P1 h9 e h10
 
-    have h11 :
-      (point, P1) :: (am' ++ (name, fun e => Typing am e t) :: am) =
-      ((point, P1) :: am') ++ (name, fun e => Typing am e t) :: am
-    := by rfl
-
-    rw [h11]
-    apply Typing.generalized_named_instantiation h1
-    {
-      simp [List.Disjoint, Prod.dom]
-      apply And.intro h7
-      simp [List.Disjoint] at h2
-      exact h2
+    rw [←List.cons_append]
+    apply Typing.generalized_named_instantiation
+    { simp [Prod.dom] at h1
+      simp [Prod.dom,h1,h5]
     }
-    { simp [Prod.dom]
-      apply And.intro
-      { intro h12 ; exact h6 (Eq.symm h12) }
+    { exact h2 }
+    { exact h3 }
+    { simp
+      apply h7 _ _ stable_P0 stable_P1 h9
+      rw [←List.cons_append]
+      apply Typing.generalized_nameless_instantiation
+      { simp [Prod.dom] at h1
+        simp [Prod.dom,h1,h5]
+      }
+      { exact h2 }
       { exact h3 }
-    }
-    { simp [Prod.dom] ; exact h4 }
-    { exact wf }
-    {
-      simp
-      apply h8 _ _ stable_P0 stable_P1 h9
-
-      have h12 :
-        (point, P0) :: (am' ++ (name, fun e => Typing am e t) :: am) =
-        ((point, P0) :: am') ++ (name, fun e => Typing am e t) :: am
-      := by rfl
-
-      rw [h12]
-      apply Typing.generalized_nameless_instantiation h1
-      {
-        simp [List.Disjoint, Prod.dom]
-        apply And.intro h7
-        simp [List.Disjoint] at h2
-        exact h2
-      }
-      { simp [Prod.dom]
-        apply And.intro
-        { intro h12 ; exact h6 (Eq.symm h12) }
-        { exact h3 }
-      }
-      { simp [Prod.dom] ; exact h4 }
-      { exact wf }
       { exact h10 }
     }
   termination_by (Typ.size body, 1)
 
   theorem MultiSubtyping.generalized_nameless_instantiation :
-    Typ.free_vars t ⊆ Prod.dom am →
-    List.Disjoint (Prod.dom am') (Prod.dom am) →
     name ∉ Prod.dom am' →
-    name ∉ Prod.dom am →
+    Typ.free_vars t = [] →
     Typ.wellformed t →
-    MultiSubtyping (am' ++ (name,fun e => Typing am e t) :: am) (Typ.constraints_instantiate depth [.var name] cs) →
-    MultiSubtyping (am' ++ (name,fun e => Typing am e t) :: am) (Typ.constraints_instantiate depth [t] cs)
-  := by cases cs with
-  | nil =>
-    simp [Typ.constraints_instantiate, MultiSubtyping, Prod.dom]
-  | cons c cs' =>
-    have (left,right) := c
-    simp [Typ.constraints_instantiate, MultiSubtyping, Prod.dom, Typ.list_prod_free_vars]
-    intro h3 h4 h5 h6 wf h7 h8
-    apply And.intro
-    { apply Subtyping.generalized_nameless_instantiation h3 h4
-      { simp [Prod.dom] ; exact h5 }
-      { simp [Prod.dom] ; exact h6 }
-      { exact wf }
-      { exact h7 }
-    }
-    { apply MultiSubtyping.generalized_nameless_instantiation h3 h4
-      { simp [Prod.dom] ; exact h5 }
-      { simp [Prod.dom] ; exact h6 }
-      { exact wf }
-      { exact h8 }
-    }
-  termination_by (List.pair_typ_size cs, 0)
-  decreasing_by
-    all_goals (apply Prod.Lex.left ; simp [List.pair_typ_size, List.pair_typ_zero_lt_size, Typ.zero_lt_size])
-
-
-  theorem MultiSubtyping.generalized_named_instantiation :
-    Typ.free_vars t ⊆ Prod.dom am →
-    List.Disjoint (Prod.dom am') (Prod.dom am) →
-    name ∉ Prod.dom am' →
-    name ∉ Prod.dom am →
-    Typ.wellformed t →
-    MultiSubtyping (am' ++ (name,fun e => Typing am e t) :: am) (Typ.constraints_instantiate depth [t] cs) →
-    MultiSubtyping (am' ++ (name,fun e => Typing am e t) :: am) (Typ.constraints_instantiate depth [.var name] cs)
+    MultiSubtyping name (am' ++ (name,fun e => Typing name [] e t) :: am) (Typ.constraints_instantiate depth [.var name] cs) →
+    MultiSubtyping name (am' ++ (name,fun e => Typing name [] e t) :: am) (Typ.constraints_instantiate depth [t] cs)
   := by cases cs with
   | nil =>
     simp [Typ.constraints_instantiate, MultiSubtyping]
   | cons c cs' =>
     have (left,right) := c
-    simp [Typ.constraints_instantiate, MultiSubtyping, Prod.dom, Typ.list_prod_free_vars]
-    intro h3 h4 h5 h6 wf h7 h8
+    simp [Typ.constraints_instantiate, MultiSubtyping]
+    intro h3 h4 h5 h6 h7
     apply And.intro
-    { apply Subtyping.generalized_named_instantiation h3 h4
-      { simp [Prod.dom] ; exact h5 }
-      { simp [Prod.dom] ; exact h6 }
-      { exact wf }
-      { exact h7 }
-    }
-    { apply MultiSubtyping.generalized_named_instantiation h3 h4
-      { simp [Prod.dom] ; exact h5 }
-      { simp [Prod.dom] ; exact h6 }
-      { exact wf }
-      { exact h8 }
-    }
+    { apply Subtyping.generalized_nameless_instantiation h3 h4 h5 h6 }
+    { apply MultiSubtyping.generalized_nameless_instantiation h3 h4 h5 h7 }
   termination_by (List.pair_typ_size cs, 0)
   decreasing_by
-    all_goals (apply Prod.Lex.left ; simp [List.pair_typ_size, List.pair_typ_zero_lt_size, Typ.zero_lt_size])
+    all_goals (apply Prod.Lex.left ; simp [Typ.zero_lt_size, List.pair_typ_size, List.pair_typ_zero_lt_size])
 
 
-  /-
-  -- NOTE:
-  -- requirement: Typ.free_vars t ⊆ Prod.dom am
-  -- ensures fresh wrt am (e.g. within universal/existential rule) is transferred to freshness wrt t
-  -- necessary, since the universal rule has no awareness of t directly
-  -/
-  -- TODO: update to make am' disjoint from Prod.dom body too
-  -- TODO: update to make name excluded disjoint from Typ.free_vars body too
-  -- TODO: to enable append/cons preservation/reflection
-  theorem Typing.generalized_nameless_instantiation :
-    Typ.free_vars t ⊆ Prod.dom am →
-    List.Disjoint (Prod.dom am') (Prod.dom am) →
+  theorem MultiSubtyping.generalized_named_instantiation :
     name ∉ Prod.dom am' →
-    name ∉ Prod.dom am →
+    Typ.free_vars t = [] →
     Typ.wellformed t →
-    Typing (am' ++ (name,fun e => Typing am e t) :: am) e (Typ.instantiate depth [.var name] body) →
-    Typing (am' ++ (name,fun e => Typing am e t) :: am) e (Typ.instantiate depth [t] body)
+    MultiSubtyping name (am' ++ (name,fun e => Typing name [] e t) :: am) (Typ.constraints_instantiate depth [t] cs) →
+    MultiSubtyping name (am' ++ (name,fun e => Typing name [] e t) :: am) (Typ.constraints_instantiate depth [.var name] cs)
+  := by cases cs with
+  | nil =>
+    simp [Typ.constraints_instantiate, MultiSubtyping]
+  | cons c cs' =>
+    have (left,right) := c
+    simp [Typ.constraints_instantiate, MultiSubtyping]
+    intro h3 h4 h5 h6 h7
+    apply And.intro
+    { apply Subtyping.generalized_named_instantiation h3 h4 h5 h6 }
+    { apply MultiSubtyping.generalized_named_instantiation h3 h4 h5 h7 }
+  termination_by (List.pair_typ_size cs, 0)
+  decreasing_by
+    all_goals (apply Prod.Lex.left ; simp [Typ.zero_lt_size, List.pair_typ_size, List.pair_typ_zero_lt_size])
+
+
+  theorem Typing.generalized_nameless_instantiation :
+    name ∉ Prod.dom am' →
+    Typ.free_vars t = [] →
+    Typ.wellformed t →
+    Typing name (am' ++ (name,fun e => Typing name [] e t) :: am) e (Typ.instantiate depth [.var name] body) →
+    Typing name (am' ++ (name,fun e => Typing name [] e t) :: am) e (Typ.instantiate depth [t] body)
   := by cases body with
   | bvar i =>
-    simp [Typ.instantiate, Prod.dom]
+    simp [Typ.instantiate]
     by_cases h0 : depth ≤ i
     { simp [h0]
       by_cases h1 : i - depth = 0
       { simp [h1]
         simp [Typ.shift_vars]
-        intro h3 h4 h5 h6 wf
+        intro h3 h4 h5
         simp [Typing]
         intro h7 P h8 h9 h10
-        rw [Prod.find_append_suffix _ _] at h9
-        {
-          simp [Prod.find] at h9
-          simp [←h9] at h10
+        rw [Prod.find_append_suffix _ h3] at h9
+        simp [Prod.find] at h9
+        simp [←h9] at h10
 
-          simp [Typ.wellformed] at wf
-          have ⟨h11,_⟩ := wf
-          rw [←Typ.instantiated_shift_vars_preservation h11]
-          apply Typing.env_append_suffix_preservation (List.disjoint_of_subset_right h3 h4)
-          apply Typing.env_cons_suffix_preservation
-          {
-            intro h12
-            specialize h3 h12
-            simp at h3
-            have ⟨P',h13⟩ := h3
-            apply h6 P' h13
-          }
-          { exact h10 }
-        }
-        { simp [Prod.dom] ; exact h5 }
+        simp [Typ.wellformed] at h5
+        have ⟨h11,_⟩ := h5
+        rw [←Typ.instantiated_shift_vars_preservation h11]
+        apply Typing.env_preservation h4 h10
       }
       { simp [h1] }
     }
     { simp [h0] }
   | var name' =>
-    simp [Typ.instantiate, Typ.free_vars, Typing, Prod.dom]
+    simp [Typ.instantiate, Typing]
   | iso l body =>
-    simp [Typ.free_vars, Typ.instantiate, Typing, Prod.dom]
-    intro h1 h2 h3 h4 wf h5
-    simp [*]
-    apply Typing.generalized_nameless_instantiation h1 h2
-    { simp [Prod.dom]; exact h3 }
-    { simp [Prod.dom]; exact h4 }
-    { exact wf }
+    simp [Typ.instantiate, Typing]
+    intro h1 h2 h3 h4 h5
+    simp [h4]
+    apply Typing.generalized_nameless_instantiation h1 h2 h3 h5
   | entry l body =>
-    simp [Typ.free_vars, Typ.instantiate, Typing, Prod.dom]
-    intro h1 h2 h3 h4 wf h5
-    simp [*]
-    apply Typing.generalized_nameless_instantiation h1 h2
-    { simp [Prod.dom]; exact h3 }
-    { simp [Prod.dom]; exact h4 }
-    { exact wf }
+    simp [Typ.instantiate, Typing]
+    intro h1 h2 h3 h4 h5
+    simp [h4]
+    apply Typing.generalized_nameless_instantiation h1 h2 h3 h5
   | path left right =>
-    simp [Typ.free_vars, Typ.instantiate, Typing, Prod.dom]
-    intro h2 h3 h4 h5 wf h6 h7
-    simp [*]
-    -- apply And.intro
-    -- { apply Typ.wellformed_nameless_instantiation h7
-    --   exact wf
-    -- }
+    simp [Typ.instantiate, Typing]
+    intro h2 h3 h4 h5 h6
+    simp [h5]
     { intro arg h9
-      apply Typing.generalized_nameless_instantiation h2 h3
-      { simp [Prod.dom]; exact h4 }
-      { simp [Prod.dom]; exact h5 }
-      { exact wf }
-      {
-        apply h7
-        apply Typing.generalized_named_instantiation h2 h3
-        { simp [Prod.dom]; exact h4 }
-        { simp [Prod.dom]; exact h5 }
-        { exact wf }
-        { exact h9 }
-      }
+      apply Typing.generalized_nameless_instantiation h2 h3 h4
+      apply h6
+      apply Typing.generalized_named_instantiation h2 h3 h4 h9
     }
   | bot =>
-    simp [Typ.free_vars, Typ.instantiate, Typing, Prod.dom]
+    simp [Typ.instantiate, Typing]
   | top =>
-    simp [Typ.free_vars, Typ.instantiate, Typing, Prod.dom]
+    simp [Typ.instantiate, Typing]
   | unio left right =>
-    simp [Typ.free_vars, Typ.instantiate, Typing, Prod.dom]
-    intro h2 h3 h4 h5 wf h6
-    cases h6 with
+    simp [Typ.instantiate, Typing]
+    intro h2 h3 h4 h5
+    cases h5 with
     | inl h7 =>
       apply Or.inl
-      apply Typing.generalized_nameless_instantiation h2 h3
-      { simp [Prod.dom]; exact h4 }
-      { simp [Prod.dom]; exact h5 }
-      { exact wf }
-      { exact h7 }
+      apply Typing.generalized_nameless_instantiation h2 h3 h4 h7
     | inr h7 =>
       apply Or.inr
-      apply Typing.generalized_nameless_instantiation h2 h3
-      { simp [Prod.dom]; exact h4 }
-      { simp [Prod.dom]; exact h5 }
-      { exact wf }
-      { exact h7 }
+      apply Typing.generalized_nameless_instantiation h2 h3 h4 h7
   | inter left right =>
-    simp [Typ.free_vars, Typ.instantiate, Typing, Prod.dom]
-    intro h2 h3 h4 h5 wf h6 h7
+    simp [Typ.instantiate, Typing]
+    intro h2 h3 h4 h5 h6
     apply And.intro
-    { apply Typing.generalized_nameless_instantiation h2 h3
-      { simp [Prod.dom]; exact h4 }
-      { simp [Prod.dom]; exact h5 }
-      { exact wf }
-      { exact h6 }
-    }
-    { apply Typing.generalized_nameless_instantiation h2 h3
-      { simp [Prod.dom]; exact h4 }
-      { simp [Prod.dom]; exact h5 }
-      { exact wf }
-      { exact h7 }
-    }
+    { apply Typing.generalized_nameless_instantiation h2 h3 h4 h5 }
+    { apply Typing.generalized_nameless_instantiation h2 h3 h4 h6 }
   | diff left right =>
-    simp [Typ.free_vars, Typ.instantiate, Typing, Prod.dom]
-    intro h2 h3 h4 h5 wf h6 h8
-    { apply And.intro
-      { apply Typing.generalized_nameless_instantiation h2 h3
-        { simp [Prod.dom]; exact h4 }
-        { simp [Prod.dom]; exact h5 }
-        { exact wf }
-        { exact h6 }
-      }
-      { intro h9
-        apply h8
-        apply Typing.generalized_named_instantiation h2 h3
-        { simp [Prod.dom]; exact h4 }
-        { simp [Prod.dom]; exact h5 }
-        { exact wf }
-        { exact h9 }
-      }
+    simp [Typ.instantiate, Typing]
+    intro h2 h3 h4 h5 h6
+    apply And.intro
+    { apply Typing.generalized_nameless_instantiation h2 h3 h4 h5 }
+    { intro h9
+      apply h6
+      apply Typing.generalized_named_instantiation h2 h3 h4 h9
     }
   | all bs cs body =>
-    simp [Typ.free_vars, Typ.instantiate]
+    simp [Typ.instantiate]
     intro h2
-    simp [Typing, Prod.dom]
-    intro h3 h4 h5 wf h6 h7 names h8 h9 h10 h11 h12
-    simp [*]
-    apply And.intro h7
+    simp [Typing]
+    intro h3 h4 h5 h6 names h7 h8 h9 h10 h11
+    simp [h5]
+    apply And.intro h6
     exists names
     simp [*]
-    intro am'' h13 h14
-
-    have h15 :
-      ∀ t' ∈ List.map Typ.var names,
-        t' = Typ.instantiate depth [t] t'
-    := by
-      intro t h15
-      have ⟨p,h16,h17⟩ := Iff.mp List.mem_map h15
-      rw [←h17]
-      simp [Typ.instantiate]
-
-    rw [Typ.list_instantiate_identity h15]
-    rw [←h8]
-    rw [←List.length_map Typ.var]
-    rw [←Typ.instantiate_zero_inside_out]
-
-    rw [←List.append_assoc]
-
-    apply Typing.generalized_nameless_instantiation
-    { exact h2 }
-    { simp [Prod.dom]; rw [h13] ; exact ⟨h11, h3⟩ }
-    { simp [Prod.dom]; simp [←h13] at h10 ; exact ⟨h10, h4⟩ }
-    { simp [Prod.dom]; exact h5 }
-    { exact wf }
+    apply And.intro
     {
-      rw [List.append_assoc]
-      rw [Typ.instantiate_zero_inside_out]
-      rw [List.length_map Typ.var]
-      rw [h8]
+      apply And.intro
+      { simp [List.Disjoint] at h9
+        simp [List.Disjoint]
+        intro name' h12 h13
+        apply h9 h12
+        apply Typ.list_prod_free_vars_instantiate_upper_bound at h13
+        simp [h3] at h13
+        apply Typ.list_prod_free_vars_instantiate_lower_bound _ _ h13
+      }
+      { simp [List.Disjoint] at h10
+        simp [List.Disjoint]
+        intro name' h12 h13
+        apply h10 h12
+        apply Typ.free_vars_instantiate_upper_bound at h13
+        simp [h3] at h13
+        apply Typ.free_vars_instantiate_lower_bound _ _ h13
+      }
+    }
+    { intro am'' h13 h14
 
-      have h16 :
+      have h15 :
         ∀ t' ∈ List.map Typ.var names,
-          t' = Typ.instantiate depth [.var name] t'
+          t' = Typ.instantiate depth [t] t'
       := by
-        intro t h16
-        have ⟨p,h17,h18⟩ := Iff.mp List.mem_map h16
-        rw [←h18]
+        intro t h15
+        have ⟨p,h16,h17⟩ := Iff.mp List.mem_map h15
+        rw [←h17]
         simp [Typ.instantiate]
 
-
-      rw [←Typ.list_instantiate_identity h16]
-      apply h12 _ h13
-      rw [←List.append_assoc]
-      rw [Typ.list_instantiate_identity h16]
-      rw [←h8]
+      rw [Typ.list_instantiate_identity h15]
+      rw [←h7]
       rw [←List.length_map Typ.var]
-      rw [←Typ.constraints_instantiate_zero_inside_out]
-      apply MultiSubtyping.generalized_named_instantiation
-      { exact h2 }
-      { simp [Prod.dom]; rw [h13] ; exact ⟨h11, h3⟩ }
-      { simp [Prod.dom]; simp [←h13] at h10 ; exact ⟨h10, h4⟩ }
-      { simp [Prod.dom]; exact h5 }
-      { exact wf }
-      { rw [List.append_assoc]
-        rw [Typ.constraints_instantiate_zero_inside_out]
-        rw [List.length_map]
-        rw [h8]
-        rw [←Typ.list_instantiate_identity h15]
-        exact h14
+      rw [←Typ.instantiate_zero_inside_out]
+
+      rw [←List.append_assoc]
+
+
+      have h2A : name ∉ Prod.dom (am'' ++ am') := by
+        simp [Prod.dom] at h2
+        simp [Prod.dom,h2]
+        rw [←h13] at h8
+        simp [Prod.dom] at h8
+        exact h8
+
+      apply Typing.generalized_nameless_instantiation
+      { exact h2A }
+      { exact h3 }
+      { exact h4 }
+      {
+        rw [List.append_assoc]
+        rw [Typ.instantiate_zero_inside_out]
+        rw [List.length_map Typ.var]
+        rw [h7]
+
+        have h16 :
+          ∀ t' ∈ List.map Typ.var names,
+            t' = Typ.instantiate depth [.var name] t'
+        := by
+          intro t h16
+          have ⟨p,h17,h18⟩ := Iff.mp List.mem_map h16
+          rw [←h18]
+          simp [Typ.instantiate]
+
+
+        rw [←Typ.list_instantiate_identity h16]
+        apply h11 _ h13
+        rw [←List.append_assoc]
+        rw [Typ.list_instantiate_identity h16]
+        rw [←h7]
+        rw [←List.length_map Typ.var]
+        rw [←Typ.constraints_instantiate_zero_inside_out]
+        apply MultiSubtyping.generalized_named_instantiation
+        { exact h2A }
+        { exact h3 }
+        { exact h4 }
+        { rw [List.append_assoc]
+          rw [Typ.constraints_instantiate_zero_inside_out]
+          rw [List.length_map]
+          rw [h7]
+          rw [←Typ.list_instantiate_identity h15]
+          exact h14
+        }
       }
     }
 
   | exi bs cs body =>
-    simp [Typ.free_vars, Typ.instantiate, Typing, Prod.dom]
-    intro h2 h3 h4 h5 wf h6 h7
-    apply And.intro h6
-    intro names h8 h9 h10 h11
-    have ⟨am'',h12A,h12B,h12C⟩ := h7 names h8 h9 h10 h11
+    simp [Typ.instantiate, Typing]
+    intro h2 h3 h4 h5 h6
+    apply And.intro h5
+    intro names h7 h8 h9 h10
+    specialize h6 names h7 h8
+    have h11A : List.Disjoint names (Typ.list_prod_free_vars (Typ.constraints_instantiate (depth + List.length bs) [Typ.var name] cs)) := by
+      simp [List.Disjoint] at h9
+      simp [List.Disjoint]
+      intro name' h11 h12
+      apply Typ.list_prod_free_vars_instantiate_upper_bound at h12
+      simp [Typ.free_vars] at h12
+      cases h12 with
+      | inl h13 =>
+        apply h9 h11
+        apply Typ.list_prod_free_vars_instantiate_lower_bound _ _ h13
+      | inr h13 =>
+        rw [h13] at h11
+        exact h8 h11
+
+    have h11B : List.Disjoint names (Typ.free_vars (Typ.instantiate (depth + List.length bs) [Typ.var name] body)) := by
+      simp [List.Disjoint] at h10
+      simp [List.Disjoint]
+      intro name' h11 h12
+      apply Typ.free_vars_instantiate_upper_bound at h12
+      simp [Typ.free_vars] at h12
+      cases h12 with
+      | inl h13 =>
+        apply h10 h11
+        apply Typ.free_vars_instantiate_lower_bound _ _ h13
+      | inr h13 =>
+        rw [h13] at h11
+        exact h8 h11
+
+    have ⟨am'',h12A,h12B,h12C⟩ := h6 h11A h11B
+
+
     exists am''
     simp [*]
     rw [←List.append_assoc]
@@ -513,23 +388,29 @@ mutual
       simp [Typ.instantiate]
 
     rw [Typ.list_instantiate_identity h14]
-    rw [←h8]
+    rw [←h7]
     rw [←List.length_map Typ.var]
+
+
+    have h2A : name ∉ Prod.dom (am'' ++ am') := by
+      simp [Prod.dom] at h2
+      simp [Prod.dom,h2]
+      rw [←h12A] at h8
+      simp [Prod.dom] at h8
+      exact h8
 
     apply And.intro
     {
       rw [←Typ.constraints_instantiate_zero_inside_out]
       apply MultiSubtyping.generalized_nameless_instantiation
-      { exact h2 }
-      { simp [Prod.dom]; rw [h12A] ; exact ⟨h11, h3⟩ }
-      { simp [Prod.dom]; simp [←h12A] at h10 ; exact ⟨h10, h4⟩  }
-      { simp [Prod.dom]; exact h5 }
-      { exact wf }
+      { exact h2A }
+      { exact h3 }
+      { exact h4 }
       {
         rw [List.append_assoc]
         rw [Typ.constraints_instantiate_zero_inside_out]
         rw [List.length_map Typ.var]
-        rw [h8]
+        rw [h7]
         rw [←Typ.list_instantiate_identity]
         { exact h12B }
         {
@@ -542,16 +423,14 @@ mutual
     }
     { rw [←Typ.instantiate_zero_inside_out]
       apply Typing.generalized_nameless_instantiation
-      { exact h2 }
-      { simp [Prod.dom]; rw [h12A] ; exact ⟨h11, h3⟩ }
-      { simp [Prod.dom]; simp [←h12A] at h10 ; exact ⟨h10, h4⟩  }
-      { simp [Prod.dom]; exact h5 }
-      { exact wf }
+      { exact h2A }
+      { exact h3 }
+      { exact h4 }
       {
         rw [List.append_assoc]
         rw [Typ.instantiate_zero_inside_out]
         rw [List.length_map Typ.var]
-        rw [h8]
+        rw [h7]
 
         rw [←Typ.list_instantiate_identity]
         { exact h12C }
@@ -565,12 +444,24 @@ mutual
     }
 
   | lfp b body =>
-    simp [Typ.free_vars, Typ.instantiate, Typing, Prod.dom]
-    intro h1 h2 h3 h4 wf h5 h6 h7
+    simp [Typ.instantiate, Typing]
+    intro h1 h2 h3 h4 h5 h6
     simp [*]
-    intro name' h8 h9 h10
+    intro name' h7 h8
+    specialize h6 name' h7
 
-    have ⟨h11A,h11B⟩ := h7 name' h8 h9 h10
+    have h9 : name' ∉ Typ.free_vars (Typ.instantiate (depth + 1) [Typ.var name] body) := by
+      intro h9
+      apply Typ.free_vars_instantiate_upper_bound at h9
+      simp [Typ.free_vars] at h9
+      cases h9 with
+      | inl h10 =>
+        apply h8
+        apply Typ.free_vars_instantiate_lower_bound _ _ h10
+      | inr h10 =>
+        apply h7 h10
+
+    have ⟨h11A,h11B⟩ := h6 h9
     apply And.intro
     {
       have h12 :
@@ -587,12 +478,10 @@ mutual
       apply PosMonotonic.generalized_nameless_instantiation
       { exact h1 }
       { exact h2 }
-      { simp [Prod.dom]; exact h3 }
-      { simp [Prod.dom]; exact h4 }
-      { exact wf }
-      { simp [Prod.dom]; exact h8 }
-      { exact h9 }
-      { simp [Prod.dom]; exact h10 }
+      { exact h3 }
+      { intro h14
+        apply h7 ((Eq.symm h14))
+      }
       {
         rw [Typ.instantiate_zero_inside_out]
         rw [h13]
@@ -621,23 +510,24 @@ mutual
       rw [←h16]
 
       have h17 :
-        (name', P) :: (am' ++ (name, fun e => Typing am e t) :: am) =
-        ((name', P) :: am') ++ (name, fun e => Typing am e t) :: am
+        (name', P) :: (am' ++ (name, fun e => Typing name [] e t) :: am) =
+        ((name', P) :: am') ++ (name, fun e => Typing name [] e t) :: am
       := by exact rfl
+
       rw [h17]
 
       rw [←Typ.instantiate_zero_inside_out]
       apply Typing.generalized_nameless_instantiation
-      { exact h1 }
-      { simp [Prod.dom]; exact ⟨h10, h2⟩ }
-      { simp [*, Prod.dom]; intro h18 ; exact h9 (Eq.symm h18) }
-      { simp [*, Prod.dom] }
-      { exact wf }
       {
-
-        have h18 :
-          (name', P) :: (am' ++ (name, fun e => Typing am e t) :: am) =
-          ((name', P) :: am') ++ (name, fun e => Typing am e t) :: am
+        simp [Prod.dom]
+        simp [Prod.dom] at h1
+        exact And.symm ⟨h1, fun h18 => h7 (Eq.symm h18)⟩
+      }
+      { exact h2 }
+      { exact h3 }
+      { have h18 :
+          (name', P) :: (am' ++ (name, fun e => Typing name [] e t) :: am) =
+          ((name', P) :: am') ++ (name, fun e => Typing name [] e t) :: am
         := by exact rfl
         rw [←h18]
         rw [Typ.instantiate_zero_inside_out]
@@ -674,25 +564,23 @@ mutual
   -- can simply use stable as a placeholder
   -/
   theorem Typing.generalized_named_instantiation :
-    Typ.free_vars t ⊆ Prod.dom am →
-    List.Disjoint (Prod.dom am') (Prod.dom am) →
     name ∉ Prod.dom am' →
-    name ∉ Prod.dom am →
+    Typ.free_vars t = [] →
     Typ.wellformed t →
-    Typing (am' ++ (name,fun e => Typing am e t) :: am) e (Typ.instantiate depth [t] body) →
-    Typing (am' ++ (name,fun e => Typing am e t) :: am) e (Typ.instantiate depth [.var name] body)
+    Typing name (am' ++ (name,fun e => Typing name [] e t) :: am) e (Typ.instantiate depth [t] body) →
+    Typing name (am' ++ (name,fun e => Typing name [] e t) :: am) e (Typ.instantiate depth [.var name] body)
   := by cases body with
   | bvar i =>
-    simp [Typ.instantiate, Prod.dom]
+    simp [Typ.instantiate]
     by_cases h0 : depth ≤ i
     { simp [h0]
       by_cases h1 : i - depth = 0
       { simp [h1]
-        intro h3 h4 h5 h6 wf h7
+        intro h3 h4 h5 h6
         simp [Typ.shift_vars]
         simp [Typing]
-        apply And.intro (Typing.safety h7)
-        exists (fun e => Typing am e t)
+        apply And.intro (Typing.safety h6)
+        exists (fun e => Typing name [] e t)
         apply And.intro
         {
           unfold Stable
@@ -702,29 +590,20 @@ mutual
           { intro h9 ; exact Typing.subject_reduction h8 h9 }
           { intro h9 ; exact Typing.subject_expansion h8 h9 }
         }
-        {
-          apply And.intro
+        { apply And.intro
           { rw [Prod.find_append_suffix _ _ ]
             { simp [Prod.find] }
-            { simp [Prod.dom];
-              intro P
-              exact h5 P
-            }
+            { exact h3 }
           }
           { simp
-            simp [Typ.wellformed] at wf
-            have ⟨h8,_⟩ := wf
-            have h9 : name ∉ Typ.free_vars t := by
-              intro h10
-              specialize h3 h10
-              simp [Prod.dom] at h3
-              have ⟨P,h11⟩ := h3
-              apply h6 P h11
-            apply Typing.env_cons_suffix_reflection h9
+            simp [Typ.wellformed] at h5
+            have ⟨h8,_⟩ := h5
 
-            apply Typing.env_append_suffix_reflection (List.disjoint_of_subset_right h3 h4)
+            apply Typing.env_reflection (by simp [h4])
+            apply Typing.env_cons_suffix_reflection (by simp [h4])
+            apply Typing.env_append_suffix_reflection (by simp [h4])
             rw [Typ.instantiated_shift_vars_preservation h8]
-            exact h7
+            exact h6
 
           }
         }
@@ -733,106 +612,93 @@ mutual
     }
     { simp [h0] }
   | var name' =>
-    simp [Typ.instantiate, Typ.free_vars, Typing, Prod.dom]
+    simp [Typ.instantiate, Typing]
   | iso l body =>
-    simp [Typ.free_vars, Typ.instantiate, Typing, Prod.dom]
-    intro h1 h2 h3 h4 wf h5
+    simp [Typ.instantiate, Typing]
+    intro h1 h2 h3 h4 h5
     simp [*]
-    apply Typing.generalized_named_instantiation h1 h2
-    { simp [Prod.dom]; exact h3 }
-    { simp [Prod.dom]; exact h4 }
-    { exact wf }
+    apply Typing.generalized_named_instantiation h1 h2 h3 h5
   | entry l body =>
-    simp [Typ.free_vars, Typ.instantiate, Typing, Prod.dom]
-    intro h1 h2 h3 h4 wf h5
+    simp [Typ.instantiate, Typing]
+    intro h1 h2 h3 h4 h5
     simp [*]
-    apply Typing.generalized_named_instantiation h1 h2
-    { simp [Prod.dom]; exact h3 }
-    { simp [Prod.dom]; exact h4 }
-    { exact wf }
+    apply Typing.generalized_named_instantiation h1 h2 h3 h5
   | path left right =>
-    simp [Typ.free_vars, Typ.instantiate, Typing, Prod.dom]
-    intro h2 h3 h4 h5 wf h6 h7
+    simp [Typ.instantiate, Typing]
+    intro h2 h3 h4 h5 h6
     simp [*]
-    { intro arg h9
-      apply Typing.generalized_named_instantiation h2 h3
-      { simp [Prod.dom]; exact h4 }
-      { simp [Prod.dom]; exact h5 }
-      { exact wf }
-      {
-        apply h7
-        apply Typing.generalized_nameless_instantiation h2 h3
-        { simp [Prod.dom]; exact h4 }
-        { simp [Prod.dom]; exact h5 }
-        { exact wf }
-        { exact h9 }
-      }
-    }
+    intro arg h9
+    apply Typing.generalized_named_instantiation h2 h3 h4
+    apply h6
+    apply Typing.generalized_nameless_instantiation h2 h3 h4 h9
+
   | bot =>
-    simp [Typ.free_vars, Typ.instantiate, Typing, Prod.dom]
+    simp [Typ.instantiate, Typing]
   | top =>
-    simp [Typ.free_vars, Typ.instantiate, Typing, Prod.dom]
+    simp [Typ.instantiate, Typing]
   | unio left right =>
-    simp [Typ.free_vars, Typ.instantiate, Typing, Prod.dom]
-    intro h2 h3 h4 h5 wf h6
-    cases h6 with
+    simp [Typ.instantiate, Typing]
+    intro h2 h3 h4 h5
+    cases h5 with
     | inl h7 =>
       apply Or.inl
-      apply Typing.generalized_named_instantiation h2 h3
-      { simp [Prod.dom]; exact h4 }
-      { simp [Prod.dom]; exact h5 }
-      { exact wf }
-      { exact h7 }
+      apply Typing.generalized_named_instantiation h2 h3 h4 h7
     | inr h7 =>
       apply Or.inr
-      apply Typing.generalized_named_instantiation h2 h3
-      { simp [Prod.dom]; exact h4 }
-      { simp [Prod.dom]; exact h5 }
-      { exact wf }
-      { exact h7 }
+      apply Typing.generalized_named_instantiation h2 h3 h4 h7
   | inter left right =>
-    simp [Typ.free_vars, Typ.instantiate, Typing, Prod.dom]
-    intro h2 h3 h4 h5 wf h6 h7
+    simp [Typ.instantiate, Typing]
+    intro h2 h3 h4 h5 h6
     apply And.intro
-    { apply Typing.generalized_named_instantiation h2 h3
-      { simp [Prod.dom]; exact h4 }
-      { simp [Prod.dom]; exact h5 }
-      { exact wf }
-      { exact h6 }
-    }
-    { apply Typing.generalized_named_instantiation h2 h3
-      { simp [Prod.dom]; exact h4 }
-      { simp [Prod.dom]; exact h5 }
-      { exact wf }
-      { exact h7 }
-    }
+    { apply Typing.generalized_named_instantiation h2 h3 h4 h5 }
+    { apply Typing.generalized_named_instantiation h2 h3 h4 h6 }
   | diff left right =>
-    simp [Typ.free_vars, Typ.instantiate, Typing, Prod.dom]
-    intro h2 h3 h4 h5 wf h7 h8
+    simp [Typ.instantiate, Typing]
+    intro h2 h3 h4 h5 h7
     apply And.intro
-    { apply Typing.generalized_named_instantiation h2 h3
-      { simp [Prod.dom]; exact h4 }
-      { simp [Prod.dom]; exact h5 }
-      { exact wf }
-      { exact h7 }
-    }
+    { apply Typing.generalized_named_instantiation h2 h3 h4 h5 }
     { intro h9
-      apply h8
-      apply Typing.generalized_nameless_instantiation h2 h3
-      { simp [Prod.dom]; exact h4 }
-      { simp [Prod.dom]; exact h5 }
-      { exact wf }
-      { exact h9 }
+      apply h7
+      apply Typing.generalized_nameless_instantiation h2 h3 h4 h9
     }
   | all bs cs body =>
-    simp [Typ.free_vars, Typ.instantiate]
+    simp [Typ.instantiate]
     intro h2
     simp [Typing, Prod.dom]
-    intro h3 h4 h5 wf h6 h7 names h8 h9 h10 h11 h12
+    intro h3 h4 h5 h6 names h7 h8 h9 h10 h11
     simp [*]
-    apply And.intro h7
+    apply And.intro h6
     exists names
     simp [*]
+    apply And.intro
+    { apply And.intro
+      { simp [List.Disjoint] at h9
+        simp [List.Disjoint]
+        intro name' h12 h13
+        apply Typ.list_prod_free_vars_instantiate_upper_bound at h13
+        simp [Typ.free_vars] at h13
+        cases h13 with
+        | inl h14 =>
+          apply h9 h12
+          apply Typ.list_prod_free_vars_instantiate_lower_bound _ _ h14
+        | inr h14 =>
+          rw [h14] at h12
+          exact h8 h12
+      }
+      { simp [List.Disjoint] at h10
+        simp [List.Disjoint]
+        intro name' h12 h13
+        apply Typ.free_vars_instantiate_upper_bound at h13
+        simp [Typ.free_vars] at h13
+        cases h13 with
+        | inl h14 =>
+          apply h10 h12
+          apply Typ.free_vars_instantiate_lower_bound _ _ h14
+        | inr h14 =>
+          rw [h14] at h12
+          exact h8 h12
+      }
+    }
     intro am'' h13 h14
 
     have h15 :
@@ -846,27 +712,28 @@ mutual
 
 
     rw [Typ.list_instantiate_identity h15]
-    rw [←h8]
+    rw [←h7]
     rw [←List.length_map Typ.var]
     rw [←Typ.instantiate_zero_inside_out]
 
     have h16A :
-      am'' ++ (am' ++ (name, fun e => Typing am e t) :: am) =
-      (am'' ++ am') ++ (name, fun e => Typing am e t) :: am
-    := by exact Eq.symm (List.append_assoc am'' am' ((name, fun e => Typing am e t) :: am))
+      am'' ++ (am' ++ (name, fun e => Typing name [] e t) :: am) =
+      (am'' ++ am') ++ (name, fun e => Typing name [] e t) :: am
+    := by exact Eq.symm (List.append_assoc am'' am' ((name, fun e => Typing name [] e t) :: am))
     rw [h16A]
 
-    apply Typing.generalized_named_instantiation
-    { exact h2 }
-    { simp [Prod.dom]; rw [h13] ; exact ⟨h11, h3⟩ }
-    { simp [Prod.dom]; simp [←h13] at h10 ; exact ⟨h10, h4⟩ }
-    { simp [Prod.dom]; exact h5 }
-    { exact wf }
-    {
-      rw [List.append_assoc]
+    have h2A : name ∉ Prod.dom (am'' ++ am') := by
+      simp [Prod.dom] at h2
+      simp [Prod.dom,h2]
+      rw [←h13] at h8
+      simp [Prod.dom] at h8
+      exact h8
+
+    apply Typing.generalized_named_instantiation h2A h3 h4
+    { rw [List.append_assoc]
       rw [Typ.instantiate_zero_inside_out]
       rw [List.length_map Typ.var]
-      rw [h8]
+      rw [h7]
 
       have h16 :
         ∀ t' ∈ List.map Typ.var names,
@@ -879,43 +746,58 @@ mutual
 
 
       rw [←Typ.list_instantiate_identity h16]
-      apply h12 _ h13
+      apply h11 _ h13
       rw [←List.append_assoc]
       rw [Typ.list_instantiate_identity h16]
-      rw [←h8]
+      rw [←h7]
       rw [←List.length_map Typ.var]
       rw [←Typ.constraints_instantiate_zero_inside_out]
       apply MultiSubtyping.generalized_nameless_instantiation
-      { exact h2 }
-      { simp [Prod.dom]; rw [h13] ; exact ⟨h11, h3⟩ }
-      { simp [Prod.dom]; simp [←h13] at h10 ; exact ⟨h10, h4⟩ }
-      { simp [Prod.dom]; exact h5 }
-      { exact wf }
+      { exact h2A }
+      { exact h3 }
+      { exact h4 }
       { rw [←h16A]
         rw [Typ.constraints_instantiate_zero_inside_out]
         rw [List.length_map]
-        rw [h8]
+        rw [h7]
         rw [←Typ.list_instantiate_identity h15]
         exact h14
       }
     }
 
   | exi bs cs body =>
-    simp [Typ.free_vars, Typ.instantiate, Typing, Prod.dom]
+    simp [Typ.instantiate, Typing]
 
-    intro h2 h3 h4 h5 wf h6 h7
-    -- simp [*]
-    -- h7 h8 h9 h10 h11 h12
-    apply And.intro h6
-    intro names h8 h9 h10 h11
-    have ⟨am'', h12A, h12B, h12C⟩ := h7 names h8 h9 h10 h11
-    clear h7
+    intro h2 h3 h4 h5 h6
+    apply And.intro h5
+    intro names h7 h8 h9 h10
+    specialize h6 names h7 h8
+
+    have h11A : List.Disjoint names (Typ.list_prod_free_vars (Typ.constraints_instantiate (depth + List.length bs) [t] cs)) := by
+      simp [List.Disjoint] at h9
+      simp [List.Disjoint]
+      intro name' h11 h12
+      apply Typ.list_prod_free_vars_instantiate_upper_bound at h12
+      simp [h3] at h12
+      apply h9 h11
+      apply Typ.list_prod_free_vars_instantiate_lower_bound _ _ h12
+
+    have h11B : List.Disjoint names (Typ.free_vars (Typ.instantiate (depth + List.length bs) [t] body)) := by
+      simp [List.Disjoint] at h10
+      simp [List.Disjoint]
+      intro name' h11 h12
+      apply Typ.free_vars_instantiate_upper_bound at h12
+      simp [h3] at h12
+      apply h10 h11
+      apply Typ.free_vars_instantiate_lower_bound _ _ h12
+
+    have ⟨am'', h12A, h12B, h12C⟩ := h6 h11A h11B
     exists am''
     apply And.intro h12A
     have h13 :
-      am'' ++ (am' ++ (name, fun e => Typing am e t) :: am) =
-      (am'' ++ am') ++ (name, fun e => Typing am e t) :: am
-    := by exact Eq.symm (List.append_assoc am'' am' ((name, fun e => Typing am e t) :: am))
+      am'' ++ (am' ++ (name, fun e => Typing name [] e t) :: am) =
+      (am'' ++ am') ++ (name, fun e => Typing name [] e t) :: am
+    := by exact Eq.symm (List.append_assoc am'' am' ((name, fun e => Typing name [] e t) :: am))
     rw [h13]
 
     have h14 :
@@ -928,23 +810,28 @@ mutual
       simp [Typ.instantiate]
 
     rw [Typ.list_instantiate_identity h14]
-    rw [←h8]
+    rw [←h7]
     rw [←List.length_map Typ.var]
+
+    have h2A : name ∉ Prod.dom (am'' ++ am') := by
+      simp [Prod.dom] at h2
+      simp [Prod.dom,h2]
+      rw [←h12A] at h8
+      simp [Prod.dom] at h8
+      exact h8
 
     apply And.intro
     {
       rw [←Typ.constraints_instantiate_zero_inside_out]
       apply MultiSubtyping.generalized_named_instantiation
-      { exact h2 }
-      { simp [Prod.dom]; rw [h12A] ; exact ⟨h11, h3⟩ }
-      { simp [Prod.dom]; simp [←h12A] at h10  ; exact ⟨h10, h4⟩ }
-      { simp [Prod.dom]; exact h5 }
-      { exact wf }
+      { exact h2A }
+      { exact h3 }
+      { exact h4 }
       {
         rw [List.append_assoc]
         rw [Typ.constraints_instantiate_zero_inside_out]
         rw [List.length_map Typ.var]
-        rw [h8]
+        rw [h7]
 
         rw [←Typ.list_instantiate_identity]
         { exact h12B }
@@ -958,16 +845,14 @@ mutual
     }
     { rw [←Typ.instantiate_zero_inside_out]
       apply Typing.generalized_named_instantiation
-      { exact h2 }
-      { simp [Prod.dom]; rw [h12A] ; exact ⟨h11, h3⟩ }
-      { simp [Prod.dom]; simp [←h12A] at h10  ; exact ⟨h10, h4⟩ }
-      { simp [Prod.dom]; exact h5 }
-      { exact wf }
+      { exact h2A }
+      { exact h3 }
+      { exact h4 }
       {
         rw [List.append_assoc]
         rw [Typ.instantiate_zero_inside_out]
         rw [List.length_map Typ.var]
-        rw [h8]
+        rw [h7]
 
         rw [←Typ.list_instantiate_identity]
         { exact h12C }
@@ -981,11 +866,22 @@ mutual
     }
 
   | lfp b body =>
-    simp [Typ.free_vars, Typ.instantiate, Typing, Prod.dom]
-    intro h1 h2 h3 h4 wf h5 h6 h7
+    simp [Typ.instantiate, Typing]
+    intro h1 h2 h3 h4 h5 h6
     simp [*]
-    intro name' h8 h9 h10
-    have ⟨h11A,h11B⟩ := h7 name' h8 h9 h10
+    intro name' h7 h8
+    specialize h6 name' h7
+
+
+    have h9 : name' ∉ Typ.free_vars (Typ.instantiate (depth + 1) [t] body)  := by
+      intro h9
+      apply Typ.free_vars_instantiate_upper_bound at h9
+      simp [h2] at h9
+      apply h8
+      apply Typ.free_vars_instantiate_lower_bound _ _ h9
+
+
+    have ⟨h11A,h11B⟩ := h6 h9
     apply And.intro
     {
       have h12 :
@@ -1000,12 +896,8 @@ mutual
       apply PosMonotonic.generalized_named_instantiation
       { exact h1 }
       { exact h2 }
-      { simp [Prod.dom]; exact h3 }
-      { simp [Prod.dom]; exact h4 }
-      { exact wf }
-      { simp [Prod.dom]; exact h8 }
-      { exact h9 }
-      { simp [Prod.dom]; exact h10 }
+      { exact h3 }
+      { intro h14 ; apply h7 ; simp [h14] }
       {
         rw [Typ.instantiate_zero_inside_out]
         rw [h13]
@@ -1033,24 +925,27 @@ mutual
       rw [←h16]
 
       have h17 :
-        (name', P) :: (am' ++ (name, fun e => Typing am e t) :: am) =
-        ((name', P) :: am') ++ (name, fun e => Typing am e t) :: am
+        (name', P) :: (am' ++ (name, fun e => Typing name [] e t) :: am) =
+        ((name', P) :: am') ++ (name, fun e => Typing name [] e t) :: am
       := by exact rfl
       rw [h17]
 
       rw [←Typ.instantiate_zero_inside_out]
       apply Typing.generalized_named_instantiation
-      { exact h1 }
-      { simp [Prod.dom]; exact ⟨h10, h2⟩ }
-      { simp [*, Prod.dom]; intro h18 ; exact h9 (id (Eq.symm h18)) }
-      { simp [*, Prod.dom] }
-      { exact wf }
+      { simp [Prod.dom]
+        simp [Prod.dom] at h1
+        simp [*]
+        intro h18
+        apply h7 ; simp [h18]
+      }
+      { exact h2 }
+      { exact h3 }
       {
 
         rw [Typ.instantiate_zero_inside_out]
         have h18 :
-          (name', P) :: (am' ++ (name, fun e => Typing am e t) :: am) =
-          ((name', P) :: am') ++ (name, fun e => Typing am e t) :: am
+          (name', P) :: (am' ++ (name, fun e => Typing name [] e t) :: am) =
+          ((name', P) :: am') ++ (name, fun e => Typing name [] e t) :: am
         := by exact rfl
         rw [←h18]
         rw [h16]
@@ -1076,76 +971,56 @@ end
 
 theorem Typing.nameless_instantiation :
   name ∉ Typ.free_vars body →
-  Typ.free_vars t ⊆ Prod.dom am →
-  name ∉ Prod.dom am →
+  Typ.free_vars t = [] →
   Typ.wellformed t →
-  Typing ((name,fun e => Typing am e t) :: am) e (Typ.instantiate depth [.var name] body) →
-  Typing am e (Typ.instantiate depth [t] body)
+  Typing name ((name,fun e => Typing name [] e t) :: am) e (Typ.instantiate depth [.var name] body) →
+  Typing name am e (Typ.instantiate depth [t] body)
 := by
-  simp [Prod.dom]
-  intro h0 h1 h2 wf h3
-  apply @Typing.env_cons_suffix_reflection _ _ _ (fun e => Typing am e t)
+  intro h0 h1 h2 h3
+  apply @Typing.env_cons_suffix_reflection _ _ _ (fun e => Typing name [] e t)
   {
     intro h5
     apply Typ.free_vars_instantiate_upper_bound at h5
-    simp at h5
-    cases h5 with
-    | inl h6 =>
-      apply h0 h6
-    | inr h6 =>
-      specialize h1 h6
-      simp at h1
-      have ⟨P,h7⟩ := h1
-      exact h2 P h7
+    simp [h1] at h5
+    apply h0 h5
   }
   {
     have h5 :
-      (name, fun e => Typing am e t) :: am =
-      [] ++ (name, fun e => Typing am e t) :: am
+      (name, fun e => Typing name [] e t) :: am =
+      [] ++ (name, fun e => Typing name [] e t) :: am
     := by rfl
     rw [h5]
-    apply Typing.generalized_nameless_instantiation h1
-    { simp [Prod.dom]}
-    { exact Iff.mp List.count_eq_zero rfl }
-    { simp [Prod.dom]; exact h2 }
-    { exact wf }
+    apply Typing.generalized_nameless_instantiation
+    { simp [Prod.dom] }
+    { exact h1 }
+    { exact h2 }
     { exact h3 }
   }
 
 theorem Typing.named_instantiation :
   name ∉ Typ.free_vars body →
-  Typ.free_vars t ⊆ Prod.dom am →
-  name ∉ Prod.dom am →
+  Typ.free_vars t = [] →
   Typ.wellformed t →
-  Typing am e (Typ.instantiate depth [t] body) →
-  Typing ((name,fun e => Typing am e t) :: am) e (Typ.instantiate depth [.var name] body)
+  Typing name am e (Typ.instantiate depth [t] body) →
+  Typing name ((name,fun e => Typing name [] e t) :: am) e (Typ.instantiate depth [.var name] body)
 := by
-  simp [Prod.dom]
-  intro h0 h1 h2 wf h3
+  intro h0 h1 h2 h3
   have h5 :
-    (name, fun e => Typing am e t) :: am =
-    [] ++ (name, fun e => Typing am e t) :: am
+    (name, fun e => Typing name [] e t) :: am =
+    [] ++ (name, fun e => Typing name [] e t) :: am
   := by rfl
   rw [h5]
-  apply Typing.generalized_named_instantiation h1
+  apply Typing.generalized_named_instantiation
   { simp [Prod.dom]}
-  { exact Iff.mp List.count_eq_zero rfl }
-  { simp [Prod.dom]; exact h2 }
-  { exact wf }
+  { exact h1 }
+  { exact h2 }
   {
     simp
-    apply Typing.env_cons_suffix_preservation _ _ (fun e => Typing am e t)
+    apply Typing.env_cons_suffix_preservation _ _ (fun e => Typing name [] e t)
     { intro h6
       apply Typ.free_vars_instantiate_upper_bound at h6
-      simp at h6
-      cases h6 with
-      | inl h7 =>
-        apply h0 h7
-      | inr h7 =>
-        specialize h1 h7
-        simp at h1
-        have ⟨P,h8⟩ := h1
-        exact h2 P h8
+      simp [h1] at h6
+      apply h0 h6
     }
     { exact h3 }
   }
